#+TITLE: Assignment 10: Vectors Part 3
* vectors at an angle
  
** a sketch
 
\begin{tikzpicture}
    \draw[black, thick, ->] (1, 0) -- (0, 1.73205080757) node[above right] {$\vec{A}$};
    \draw[black, thick, ->] (1, 0) -- (0, 0) node[above left] {$\text{proj}_{\vec{B}} \vec{A}$};
    \draw[black, thick, ->] (1, 0) -- (7, 0) node[above right] {\( \vec{B} \)};
    \draw[black, thick, ->] (1, 0) -- (2.5, -2.598) node[above right] {$\text{proj}_{\vec{A}} \vec{B}$};
\end{tikzpicture}

** components
   
   \[\begin{aligned}
   \text{comp} _{\vec{A}} \vec{B} &= 6 \cos  120 ^\circ \\
   \text{comp} _{\vec{B}} \vec{A} &= 2 \cos  120 ^\circ \\
   \end{aligned}\]

** dot product

   
   \[\begin{aligned}
   \vec{A} \cdot \vec{B} &= |A| |B| \cos  \theta \\
   &= 2 \cdot 6 \cdot \cos  120 = -6
   \end{aligned}\]
   
* proving expression for component 
  
  Lets redefine the coordinate axis so that $\vec{A}$ lies along the x-axis. Then,
  \[\begin{aligned}
  \text{comp}_{\vec{A}} \vec{B} &= |\vec{B}| \cos  \theta \\
  &= \frac{ |\vec{A}| |\vec{B}| \cos  \theta }{| \vec{A}|}\\
  &= \frac{ \vec{A} \cdot \vec{B}}{|\vec{A}|}
  \end{aligned}\]
  
* expression for projection

  The projection is just a vector with length $\text{comp}_{\vec{A}} \vec{B}$ in the direction of $\vec A$.
  
  \[\begin{aligned}
  \left( \frac{\vec{A} \cdot \vec{B}}{|\vec{A}|} \right)  \frac{\vec{A}}{|\vec{A}|}
  \end{aligned}\]
  
* expression for perpendicular
  The part of $\vec{A}$ that is perpendicular to $\vec B$ is just the whole vector minus the part that is parallel:
  
  \[\begin{aligned}
  \vec{A}_{\perp  \vec{B}} &= \vec{A} - \text{proj}_{\vec{B}} \vec{A}\\
  &= \vec{A} - \left( \frac{ \vec{A} \cdot \vec{B} }{|\vec{B}|^2} \right)  \vec{B}\\
  \end{aligned}\]

  Checking using the dot product:

  
  \[\begin{aligned}
  \left(  \vec{A} - \left( \frac{ \vec{A} \cdot \vec{B} }{|\vec{B}|^2} \right)  \vec{B} \right)  \cdot \vec{B} &= \vec{A} \cdot \vec{B} - \left( \frac{ \vec{A} \cdot \vec{B} }{|\vec{B}|^2} \right)  \vec{B} \cdot \vec{B}\\
  &= \vec{A} \cdot \vec{B} - \left( \frac{ \vec{A} \cdot \vec{B} }{|\vec{B}|^2} \right)  |\vec{B}|^2\\
  &= \vec{A} \cdot \vec{B} - \vec{A} \cdot \vec{B} \\
  &= 0
  \end{aligned}\]

  
* find angle using dot product
  
  Well, the dot product already includes the angle, so let's just solve for that
  \[\begin{aligned}
  \cos \theta &= \frac{ \vec{A} \cdot \vec{B} }{|\vec{A}| |\vec{B}|}
  \end{aligned}\]

  The angle between:
  
  \[\begin{aligned}
  \theta &= \cos  ^- \left( \frac{3 + 2 - 4}{\sqrt{1^2 + 2^2 + 2^2} \sqrt{3^2 + 1^2 + 2^2}}\right)  \\
  &= \cos  ^-  \left( (3 + 2 - 4) / (3 * \sqrt{14}) \right)= \cos  ^- ( 0.08908708 ) &\approx 84.8 ^\circ
  \end{aligned}\]

  
  
* distributivity of dot product across vector addition
  The dot product is defined as 
  \[\begin{aligned}
  \vec{A} \cdot \vec{B} &= |\vec{A}| |\vec{B}| \cos \theta \\
  &= |\vec{A}| \text{comp}_{\vec{A}} \vec{B}
  \end{aligned}\]

  We want to show that
  
  \[\begin{aligned}
  \vec{A} \cdot \left( \vec{B} + \vec{C} \right) &= \vec{A} \cdot \vec{B} + \vec{A} \cdot \vec{C}\\
  \end{aligned}\]

  
  \[\begin{aligned}
  \vec{A} \cdot \left( \vec{B} + \vec{C} \right)
  &= | \vec{A} | \text{comp}_{\vec{A}}  \left( \vec{B} + \vec{C} \right)  \right)\\
  &= | \vec{A} | \left( \text{comp}_{\vec{A}} \vec{B} + \text{comp}_{\vec{A}} \vec{C} \right) &&\quad\ \text{distributivity of components over addition}\\
  &= | \vec{A} |\text{comp}_{\vec{A}} \vec{B} + | \vec{A} |\text{comp}_{\vec{A}} \vec{C}\\
  &= \vec{A} \cdot \vec{B} + \vec{A} \cdot \vec{C}
  \end{aligned}\]

  Distributivity of component addition can be seen by imagining a new coordinate system where $\vec A$ is one of the axes. The amount that each vector "moves a spot" along a direction combined is the same as if you did the moves separately. 
  
* line through a point
  

  
  \[\begin{aligned}
  \vec{r}(t) &= \vec{P_0} + \vec{v_0} t
  \end{aligned}\]

  This way, $\vec r(t) = \vec{P_0}$ at $t = 0$, and the direction of the line is the velocity vector ($\frac{d}{dt}\vec{r} = \vec{v_0}$).


* vector equation that passes through the points

  The vectors are 
  \[\begin{aligned}
  \vec{a} &= \langle -1, 4, 1 \rangle \\
  \vec{b} &= \langle 2, -5, -3 \rangle
  \end{aligned}\]

  Let's choose 
  \[\begin{aligned}
  \vec{r}(t) &= \vec{p} + \vec{v}t\\
  \end{aligned}\]
   and make sure that $\vec{r}(0) = \vec{a}$, and $\vec{r}(1) = \vec{b}$.
  We can do this by setting 
  \[\begin{aligned}
  \vec{p} &= \vec{a} = \langle -1, 4, 1 \rangle\\
  \vec{v} &= \vec{b} - \vec{a} = \langle 3, -9, -4 \rangle
  \end{aligned}\]

  Thus,
\[\begin{aligned}
\boxed{\vec{r}(t) = \langle -1, 4, 1 \rangle + \langle 3, -9, -4 \rangle t}
\end{aligned}\]


  This way, 
  \[\begin{aligned}
  \vec{r}(0) &= \vec{p} = \vec{a}\\
  \vec{r}(1) &= \vec{p} + \vec{v} = \vec{a} + (\vec{b} - \vec{a}) = \vec{b}
  \end{aligned}\]
