#+TITLE: Assignment 3: arclength
* shoestring loop
  
  \[\begin{aligned}
  x &= t^2\\
  y &= t^3-3t\\
  \frac{dx}{dt} &= 2t\\
  \frac{dy}{dt} &= 3t^2-3\\
  \frac{dy}{dx} &= \frac{3t^2-3}{2t}
  \end{aligned}\]
** tangents are horizontal or vertical
*** horizontal
    
    \[\begin{aligned}
    3t^2-3 &= 0\\
    3t^2 &= 3\\
    t^2 &= 1\\
    t &= \pm 1
    \end{aligned}\]

    Now, let's find the actual coordinates
    
    \[\begin{aligned}
    x &= t^2 &&= 1\\
    y &= t^3-3t &&= -2 \text{ or } 2
    \end{aligned}\]
    and it checks out graphically.


*** vertical
    
    
    \[\begin{aligned}
    2t &= 0\\
    t &= 0\\
    \end{aligned}\]

    The actual coordinates
    
    \[\begin{aligned}
    (t^2, t^3-3t) = (0, 0)
    \end{aligned}\]
    and it checks out graphically.


** concave up
   
   \[\begin{aligned}
   \frac{d}{dx} \frac{dy}{dx} = \frac{\dot{x}\ddot{y}-\dot{y}\ddot{x}}{\dot{x}^3} = \frac{2t(6t)-(3t^2-3)(2)}{8t^3}\\
   = \frac{6t^2-3t^2+3}{4t^3} = \frac{3t^2+3}{4t^3} > 0\\
   \therefore \text{concave up for }t > 0
   \end{aligned}\]

** concave down

   Using similar logic, the curve is concave down for $t \le 0$.

   
* polar curves + converting to cartesian 

  [[file:KBe21math520retAssign3polarSketches.png]]

  Also see the (updated) [[https://www.desmos.com/calculator/jah3gjef7y][desmos]].
  
 \setcounter{section}{3}
* cardiod

** sketch
   [[file:KBe21math520retAssign3cardiodSketch.png]]
   
** crosses the origin
   Only hapens when $\theta = 0$.
   
   \[\begin{aligned}
   r = 1 + 2 \cos  \theta  &= 0\\
   2 \cos  \theta  &= -1\\
   \cos  \theta &= -\frac{1}{2}\\
   \theta &= \cos ^-  \left(-\frac{1}{2}\right)  \\
   &= \frac{2\pi}{3}, -\frac{2\pi}{3}
   \end{aligned}\]

   
** derivatives to verify crossing

   Let's choose the crossing $\theta  = \frac{2\pi}{3}$
   
   \[\begin{aligned}
   y &= r \sin  \theta  = (1 + 2 \cos  \theta) \sin  \theta = \sin  \theta + 2 \cos  \theta  \sin  \theta = \sin  \theta  + \sin  2\theta\\
   x &= r \cos  \theta  = (1 + 2 \cos  \theta ) \cos \theta = \cos  \theta  + 2 \cos^2 \theta  \\
   \frac{dy}{d\theta } &= \cos  \theta  + 2 \cos 2 \theta \implies -\frac{1}{2} + 2\left(-\frac{1}{2}\right)= - \frac{3}{2}\\
   \frac{dx}{d\theta } &= -\sin  \theta - 2 (2 \cos  \theta ) \sin \theta = - \sin  \theta - 2 \sin  2 \theta = -\frac{\sqrt{3}}{2} - 2 (- \frac{\sqrt{3}}{2}) = \frac{\sqrt{3}}{2}\\
   \frac{d^2y}{d\theta ^2} &= -\sin  \theta - 4 \sin  2 \theta = -\frac{\sqrt{3}}{2} - 4  \left( -\frac{\sqrt{3}}{2} \right) = 3 \frac{\sqrt{3}}{2} \\
   \frac{d^2x}{d\theta ^2} &= -\cos \theta - 4 \cos  2 \theta = \frac{5}{2}\\
   \frac{dy}{dx} &= \frac{\dot{y}}{\dot{x}} = -\frac{ \cos  \theta + 2 \cos 2 \theta}{\sin  \theta + 2 \sin  2 \theta } = -\frac{\frac{3}{2}}{\frac{\sqrt{3}}{2}} = -\sqrt{3}\\
   \frac{dy^2}{dx^2} &= \frac{\dot{x}\ddot{y} - \ddot{x}\dot{y}}{\dot{x}^3} = \frac{ \frac{\sqrt{3}}{2} 3\frac{\sqrt{3}}{2} + \frac{5}{2} \frac{3}{2} }{\left(\frac{\sqrt{3}}{2}\right)^3}\\
   &= \frac{\frac{9}{4}+\frac{15}{4}}{\frac{3\sqrt{3}}{8}} &= \frac{24}{4} \frac{8}{3\sqrt{3}} = -\frac{16}{\sqrt{3}}
   \end{aligned}\]
   
** points where tangent is horizontal or vertical
   
*** horizontal
    
    
    \[\begin{aligned}
    \frac{dy}{dx} &= \frac{\cos  \theta  + 2 \cos 2 \theta }{\sin  \theta  + 2 \sin  2 \theta } &= 0\\
    \implies&  \cos  \theta  + 2 \cos  2 \theta  &= 0\\
    & \cos  \theta + 2 \cos  ^2 \theta  - 2 \sin  ^2 \theta  &= 0\\
    \end{aligned}\]
    
    \[\begin{aligned}
    0 &= \cos  \theta  + 2 \cos  ^2 \theta  - 2 \sin  ^2 \theta\\
    0 &= \cos  \theta  + 2 \cos  ^2 \theta  - 2 \left(1-\cos  ^2 \theta\right)\\
    0 &= \cos  \theta  + 2 \cos  ^2 \theta  - 2 + 2 \cos  ^2 \theta\\
    0 &= 4 \cos  ^2 \theta  + \cos  \theta - 2\\
    \cos  \theta  &= \frac{-1 \pm \sqrt{1+4(4)2}}{8} = \frac{-1 \pm \sqrt{33}}{8}
    \end{aligned}\]

    
    \[\begin{aligned}
    \theta &= \cos  ^{-1} \left( \frac{-1 + \sqrt{33}}{8} \right), \cos  ^{-1} \left( \frac{-1-\sqrt{33}}{8} \right)  \\
    &= 0.936, 3.709, 2.574, 5.347\\
    &= (1.296, 1.76), (0.579, 0.369), (0.579, 0.369), (1.296, -1.76)
    \end{aligned}\]

    
*** vertical

    
    \[\begin{aligned}
    \frac{dx}{dy} &= \frac{ \sin  \theta  + 2 \sin  2 \theta }{\cos  \theta  + 2 \cos  2 \theta }\\
    \implies  &\ \quad \sin  \theta  + 2 \sin  2 \theta = 0
    \end{aligned}\]

    Make sure the top isn't also zero when the bottom is zero. Otherwise, by L'hospital rule that $\frac{0}{0}$ could be anything in the world. 
    
    \[\begin{aligned}
    0 &= \sin  \theta  + 2 \sin  2 \theta \\
    &= \sin  \theta  + 4 \sin  \theta \cos  \theta \\
    &= \sin  \theta  (1+4 \cos  \theta )\\
    \end{aligned}\]

    Either $\theta = 0, \pi$, or 
    
    \[\begin{aligned}
    0 &= 1+4 \cos  \theta \\
    -\frac{1}{4} &= \cos  \theta \\
    \theta &= 1.823, 4.46\\
    \end{aligned}\]

    The locations are at $(1, 0), (3, 0), (-0.125, -0.4847), (-0.125, 0.4847)$.
    
** tangent line
   
   \[\begin{aligned}
   y=-\sqrt{3}x
   \end{aligned}\]

   
* arclength
  
  \[\begin{aligned}
  S = \int_{C} ds = \lim_{n \to  \infty} \sum_{i=1}^{n}  \sqrt{\Delta x_i^2 + \Delta  y_i^2}
  \end{aligned}\]

  Also note that 
  \[\begin{aligned}
  \boxed{\frac{dy}{dx} \triangleq \lim_{\Delta x \to  0} \frac{\delta y}{\delta x}}
  \end{aligned}\]


  
** if $y = f(x)$
   
   \[\begin{aligned}
   S &= \lim_{n \to  \infty} \sum_{i=1}^{n} \sqrt{ \left( \frac{dx^2}{dx^2} + \frac{dy^2}{dx^2} \right) dx^2 }  \\
   &= \lim_{n \to  \infty} \sum_{i=1}^{n} \sqrt{\frac{dx^2}{dx^2} + \frac{dy^2}{dx^2}} dx \\
   &= \lim_{n \to  \infty} \sum_{i=1}^{n} \sqrt{1 + \left( \frac{dy}{dx} \right)  ^2} dx \\
   \end{aligned}\]

** if $y = y(t), x = x(t)$
   
   \[\begin{aligned}
   \Delta S &= \sqrt{\Delta x^2 + \Delta y^2} \frac{\Delta t}{\Delta t}\\
   \implies & \ \quad \sqrt{\frac{\Delta x^2}{\Delta t^2} + \frac{\Delta y^2}{\Delta t^2}} \Delta t\\
   \implies & \ \quad  \int \sqrt{\frac{dx^2}{dt^2} + \frac{dy^2}{dt^2}} dt
   \end{aligned}\]


