#+TITLE: Assignment 10
#+AUTHOR: Peter Choi

* Problem 1:
** 1.1)
#+DOWNLOADED: screenshot @ 2021-11-01 13:15:52
[[file:2021-11-01_13-15-52_screenshot.png]]
** 1.2)
$comp_{\vec A}\vec B=|\vec B|\cos(\theta)=6\cos(\frac{2\pi}{3})=-3$
$comp_{\vec B}\vec A=|\vec A|\cos(\theta)=2\cos(\frac{2\pi}{3})=-1$
** 1.3)
$\begin{equation*}\vec A\cdot \vec B\newline = |\vec A||\vec B|\cos(\theta)=6\cdot2\cdot(-0.5)\newline=-6\end{equation*}$
* Problem 2:
$\begin{equation*}
comp_{\vec A}\vec B= |\vec B|\cos(\theta)\newline
= |\vec B|\cos(\theta)\times\frac{|\vec A|}{|\vec A|}\\
= \frac{|\vec A||\vec B|\cos(\theta)}{|\vec A|}\\
= \frac{\vec A\cdot \vec B}{|\vec A|}
\end{equation*}$

* Problem 3:
The projection of $\vec B$ onto $\vec A$ would be the $\vec A$ component of $\vec B$ times the unit vector of $\vec A$ to give the component a direction and make it a vector:
$\begin{equation*}
\vec{proj}_{\vec A} \vec B=comp_{\vec A}\vec B\cdot\hat A\\
=|\vec B|\cos(\theta)\cdot\frac{\vec A}{|\vec A|}\\
=\frac{|\vec B|\cos(\theta)}{|\vec A|}\vec A
\end{equation*}$

* Problem 4:
Because of vector addition we know that:

$$\vec A_{\perp\vec B}=\vec A-\vec A_{\parallel\vec B}$$

and thus:

$\begin{equation*}
=\vec A-|\vec A|\cos(\theta)\hat B\\
=\vec A-\frac{|\vec A|\cos(\theta)}{|\vec B|}\vec B\\
=\vec A-\frac{\vec A\cdot\vec B}{|\vec B|^2}\vec B
\end{equation*}$

We can check this by taking the dot product of the vector above and $\vec B$. If the dot product equals zero then the two vectors apre perpendicular:

$$\vec B\cdot\vec A_{\perp\vec B}=\vec B\cdot(\vec A-\frac{\vec A\cdot\vec B}{|\vec B|^2}\vec B)$$

from problem 7 we know that the dot product is distributive, and thus:

$\begin{equation*}
=\vec A\cdot\vec B-\vec A\cdot\vec B\frac{1}{|\vec B|^2}\cdot\vec B\cdot\vec B\\
=\vec A\cdot\vec B-\vec A\cdot\vec B\frac{1}{|\vec B|^2}\cdot|\vec B||\vec B|\cos(0)\\
=\vec A\cdot\vec B-\vec A\cdot\vec B\frac{1}{|\vec B|^2}\cdot|\vec B|^2\\
=\vec A\cdot\vec B-\vec A\cdot\vec B\frac{|\vec B|^2}{|\vec B|^2}\\
=\vec A\cdot\vec B-\vec A\cdot\vec B\\
=0
\end{equation*}$

* Problem 5:
The dot product is defined as:

$$\vec A\cdot\vec B=|\vec A||\vec B|\cos(\theta)$$

is this case we can solve for theta:

$\begin{equation*}
\vec A\cdot\vec B=|\vec A||\vec B|\cos(\theta)\\
\Rightarrow\frac{\vec A\cdot\vec B}{|\vec A||\vec B|}=\cos(\theta)\\
\Rightarrow \theta = \cos^-(\frac{\vec A\cdot \vec B}{|\vec A||\vec B|})
\end{equation*}$

because we do not know theta we can use another definition of the dot product to get the numorator of the fraction:

$\Rightarrow \theta=\cos^-(\frac{A_xB_x+A_yB_y+A_zB_z}{|\vec A||\vec B|})$

Therefore the angle between the two vectors $(-1,2,-2)$ and $(-3,1,2)$ is the following:

$\begin{equation*}\theta =\cos^-( \frac{3+2-4}{\sqrt{1+4+4}\cdot\sqrt{9+1+4}})\\
\Rightarrow\theta =\cos^-( \frac{1}{3\sqrt{14}})\\
\Rightarrow\theta\approx1.48159
\end{equation*}$

* Problem 6:

#+DOWNLOADED: screenshot @ 2021-11-02 22:50:57
[[file:2021-11-02_22-50-57_screenshot.png]]


Looking at the diagram above we see that:

$\begin{equation*}
proj_{\vec C}\vec A+proj_{\vec C}\vec B=proj{\vec C}(\vec A+\vec B)\\
\Rightarrow |\vec C|proj_{\vec C}\vec A+|\vec C|proj_{\vec C}\vec B=|\vec C|proj_{\vec C}(\vec A+\vec B)\\
\Rightarrow  |\vec C||\vec A|\cos(\theta_{\vec A})+|\vec C||\vec B|\cos(\theta_{\vec B})=|\vec C||\vec A+\vec B|\cos(\theta_{\vec A+\vec B})\\
\Rightarrow \vec C\cdot \vec A+\vec C\cdot\vec B=\vec C\cdot(\vec A+\vec B)
\end{equation*}$

thus the dot product is distributive

this scales to the third dimention, because in a sense the diagram is the projection of 3D vectors onto a plane. 

* Problem 7:
$\begin{equation*}
\vec A \cdot\vec B = (A_x\hat i+A_y\hat j+A_z\hat k)\cdot(B_x\hat i+B_y\hat j+ B_z\hat k)\\
= A_x\hat i\cdot B_x\hat i+ A_x\hat i\cdot B_y\hat j+ A_x\hat i\cdot B_z\hat k+A_y\hat j\cdot B_x\hat i+ A_y\hat j\cdot B_y\hat j+A_y\hat j\cdot B_z\hat k+A_z\hat k\cdot B_x\hat i+ A_z\hat k\cdot B_y\hat j+A_z\hat k\cdot B_z\hat k
\end{equation*}$

the dot product between $A_x\hat i\cdot B_x\hat i$ would be: $|A_x||B_x|\cos(0)$, because the angle between $\hat i$ and $\hat i$ is $0$ (they have the same direction), $\cos(0)=1$, and thus the dot product equals $A_xB_x$. However, the dot product between and two unit vectors that are not the same would yield a theta of $\pi\over2$, which means $\cos({\pi\over2}) = 0$ and thus that term would equal zero. This can be generalized as, if the two unit vectors are the same then it will yield a term equal to the product of their two coefficients, and if the two unit vectors are different, then the resulting term would be equal to zero. Therefore:

$\begin{equation*}=A_xB_x+0+0+A_yB_y+0+0+A_zB_z+0+0\\
=A_xB_x+A_yB_y+A_zB_z\end{equation*}$

* Problem 8:
$$\{\vec r=\vec P_o+t(\vec v_o),t\in\mathbb{R}\}$$

this works because the $\vec P_o$ term will position the vector so that the line passes through the point $\vec P_o$, and then the $t(\vec v_o)$ term will add and subtract and infinite amount of vectors in the direction and of the magnitude of $t(\vec v_o)$ from $\vec P_o$, thus creating a line that passes through $\vec P_o$ 

* Problem 9:
This is pretty similar to problem 8, the only differenc is that the $\vec P_o$ now equals one of the give vectors, and $\vec v_o$ is the vector between the two points:

$\begin{equation*}
\{\vec r=\langle2,-5,-3\rangle+t\langle1,-9,-4\rangle,t\in\mathbb{R}\}=\{\vec r=\langle2,-5,-3\rangle+\langle t,-9t,-4t\rangle,t\in\mathbb{R}\}\\
= \{\vec r=\langle2+t,-5-9t,-3-4t\rangle,t\in\mathbb{R}\}
\end{equation*}$

* Problem 10:
The law of cosines is as follows:

$$c^2=a^2+b^2-2ab\cos(\theta)$$

If the vectors $\vec c, \vec a$ and $\vec b$ are the legs of the triangle then $c,a$ and $b$ are the magnitudes of the vectors respectively, and $\theta$ is the angle between vectors $\vec a$ and $\vec b$ tail to tail


#+DOWNLOADED: screenshot @ 2021-11-03 19:42:01
[[file:2021-11-03_19-42-01_screenshot.png]]


looking at the image above we see that:

$\begin{equation*}\vec c=\vec a-\vec b\\
\Rightarrow \langle c_x,c_y,c_z\rangle=\langle a_x,a_y,a_z\rangle-\langle b_x,b_y,b_z\rangle\\
\Rightarrow \langel c_x,c_y,c_z\ranle=\langle a_x-b_x,a_y-b_y,a_z-b_z\rangle
\end{equation}$

We also know that by the definition of a vector:

$$\vec a=\langle a_x,a_y,a_z\rangle$$

$$\vec b=\langle b_x,b_y,b_z\rangle$$

We can use these numbers and plug them into the the law of cosines:

$\begin{equation*}
c^2=a^2+b^2-2ab\cos(\theta)\\
\Rightarrow|\vec c|=|\vec a|^2+|\vec b|^2-2|\vec a||\vec b|\cos(\theta)\\
\Rightarrow c_x^2+c_y^2+c_z^2=a_x^2+a_y^2+a_z^2+b_x^2+b_y^2+b_z^2-2|\vec a||\vec b|\cos(\theta)\\
\Rightarrow (a_x-b_x)^2+(a_y-b_y)^2+(a_z-b_z)^2=a_x^2+a_y^2+a_z^2+b_x^2+b_y^2+b_z^2-2|\vec a||\vec b|\cos(\theta)\\
\Rightarrow a_x^2-2a_xb_x+bx^2+a_y^2-2a_yb_y+b_y^2+a_z^2+2a_zb_z+b_z^2=a_x^2+a_y^2+a_z^2+b_x^2+b_y^2+b_z^2-2|\vec a||\vec b|\cos(\theta)\\
\Rightarrow -2a_xb_x-2a_yb_y-2a_zb_z=-2|\vec a||\vec b|\cos(\theta)\\
\Rightarrow -2(a_xb_x+a_yb_y+a_zb_z)=-2|\vec a||\vec b|\cos(\theta)\\
\Rightarrow a_xb_x+a_yb_y+a_zb_z=|\vec a||\vec b|\cos(\theta)
\end{equation*}$
