:PROPERTIES:
:ID:       B77E9C36-F22F-4F03-B935-34A7E824AE14
:END:

#+TITLE: Launchers

\begin{align*}
\Delta \text{PE} = \text{PE}_H - \text{PE}_{h_0} \\
\text{PE}_H = mgH \\
\text{PE}_{h_0} = mgh_0\\
\Delta \text{PE} = mg(H-h_0) \\
\end{align*}




\begin{align*}
\Delta\text{PE} = \text{KE} \\
mg(H-h_0)  = \frac{1}{2} mv^2 \\
g(H-h_0)  = \frac{1}{2} v^2 \\
\sqrt{2g(H-h_0)}  = v \\
\end{align*}


\begin{cases}
x(t_f) = x_f = v_0\cos\theta t_f = \sqrt{2g(H-h_0)}\cos\theta t_f\\
y(t_f) = 0 =  v_0\sin\theta t_f - \frac{1}{2}gt_f^2 + h_0 = \sqrt{2g(H-h_0)}\sin\theta t_f - \frac{1}{2}gt_f^2 + h_0\\
\end{cases}


# $t_f = \frac{-v_0\sin\theta \pm \sqrt{v_0^2\sin^2\theta + 2gh_0}}{-g} = \frac{v_0\sin\theta \pm \sqrt{v_0^2\sin^2\theta + 2gh_0}}{g}$

# Since time has to be positive, we can take the $+$ solution.
# $t_f = \frac{v_0\sin\theta + \sqrt{v_0^2\sin^2\theta + 2gh_0}}{g}$

# \begin{align*}
# x_f =v_0\cos\theta  \frac{v_0\sin\theta + \sqrt{v_0^2\sin^2\theta + 2gh_0}}{g} \\
# x_f =v_0\cos\theta  \frac{v_0\sin\theta + \sqrt{v_0^2\sin^2\theta + 2gh_0}}{g} \\
# \end{align*}


$\frac{x_f}{v_0 \cos\theta} =  t_f$

We can then plug this in and apply implicit differentiation to get $\frac{dx_f}{d\theta}$:
\begin{align*}
0 = - \frac{1}{2}g\left(\frac{x_f}{v_0\cos\theta}\right)^2 + v_0\sin\theta \frac{x_f }{v_0 \cos\theta} + h_0 \\
\frac{d}{d\theta}  0 = \frac{d}{d\theta}\left( - \frac{1}{2}g\left(\frac{x_f}{v_0\cos\theta}\right)^2\right) + \frac{d}{d\theta} v_0\sin\theta \frac{x_f }{v_0 \cos\theta} + \frac{d}{d\theta}  h_0 \\
0 = \frac{d}{d\theta}\left( - \frac{1}{2}g\left(\frac{x_f}{v_0\cos\theta}\right)^2\right) + \frac{d}{d\theta} \tan\theta x_f + 0\\
0 = \frac{d}{d\theta}\left( - \frac{1}{2}g\frac{x_f^2}{v_0^2\cos^2\theta}\right) + \frac{d}{d\theta} \tan\theta x_f + 0\\
0 = \frac{d}{d\theta}\left( - \frac{1}{2v_0^2}gx_f^2\frac{1}{\cos^2\theta}\right) + \frac{d}{d\theta} \tan\theta x_f \\
0 = - \frac{g}{2v_0^2} \frac{d}{d\theta}\left( x_f^2\frac{1}{\cos^2\theta}\right) + \frac{d}{d\theta}\tan\theta x_f \\
0 = - \frac{g}{2v_0^2} \left( 2x_f\frac{dx_f}{d\theta}\frac{1}{\cos^2\theta} + x_f^2 2\tan\theta\sec^2\theta  \right)\frac{1}{\cos^2\theta}\right) \sec^2\theta x_f + \tan\theta \frac{dx_f}{d\theta} \\
\end{align*}



\begin{align*}
0 = - \frac{g}{2v_0^2}2x_f\frac{dx_f}{d\theta}\frac{1}{\cos^2\theta} - \frac{g}{2v_0^2} x_f^2 2\tan\theta\sec^2\theta + \sec^2\theta x_f + \tan\theta \frac{dx_f}{d\theta} \\
\frac{g}{2v_0^2} 2x_f^2 \tan\theta\sec^2\theta - \sec^2\theta x_f = - \frac{g}{2v_0^2}2x_f\frac{dx_f}{d\theta}\frac{1}{\cos^2\theta} + v_0\tan\theta \frac{dx_f}{d\theta} \\
\frac{g}{2v_0^2} 2x_f^2 \tan\theta\sec^2\theta - \sec^2\theta x_f = \frac{dx_f}{d\theta} \left( v_0 \sec^2\theta x_f - \frac{g}{2v_0^2}2x_f\frac{1}{\cos^2\theta} \right ) \\
\frac{\frac{g}{2v_0^2} 2x_f^2 \tan\theta\sec^2\theta - \sec^2\theta x_f}{v_0 \sec^2\theta x_f - \frac{g}{2v_0^2}2x_f\frac{1}{\cos^2\theta} \right} = \frac{dx_f}{d\theta}  \\
\end{align*}

We can now optimize this monstrosity:
\begin{align*}
\frac{\frac{g}{2v_0^2} 2x_f^2 \tan\theta\sec^2\theta - \sec^2\theta x_f}{v_0 \sec^2\theta x_f - \frac{g}{2v_0^2}2x_f\frac{1}{\cos^2\theta} \right} = 0 \\
\end{align*}
\begin{align*}
\frac{g}{2v_0^2} 2x_f^2 \tan\theta\sec^2\theta -  \sec^2\theta x_f = 0 \\
\frac{g}{2v_0^2} 2x_f^2 \tan\theta\sec^2\theta -  \sec^2\theta x_f = 0 \\
\frac{g}{2v_0^2} 2x_f^2 \tan\theta\sec^2\theta = \sec^2\theta x_f \\
\frac{g}{v_0^2} x_f\tan\theta = 1 \\
\tan\theta = \frac{1}{x_f} \frac{v_0^2}{g} \\
\tan\theta = \frac{v_0^2}{gx_f} \\
\end{align*}

\begin{align*}
0 = - \frac{1}{2}g\left(\frac{x_f}{v_0\cos\theta}\right)^2 + v_0\sin\theta \frac{x_f }{v_0 \cos\theta} + h_0 \\
0 = - \frac{1}{2}g\frac{x_f^2}{v_0^2}\frac{1}{\cos^2\theta} + x_f \tan\theta + h_0 \\
0 = - \frac{1}{2}g\frac{x_f^2}{v_0^2}(1+\tan^2\theta) + x_f \tan\theta + h_0 \\
0 = - \frac{1}{2}g\frac{x_f^2}{v_0^2}\left(1+\frac{v_0^4}{g^2x_f^2}\right) + x_f \frac{v_0^2}{gx_f} + h_0 \\
0 = - \frac{1}{2}g\frac{x_f^2}{v_0^2}-\frac{1}{2}g\frac{x_f^2}{v_0^2}\frac{v_0^4}{g^2x_f^2} + \frac{v_0^2}{g} + h_0 \\
0 = - \frac{1}{2}g\frac{x_f^2}{v_0^2}-\frac{1}{2}\frac{v_0^2}{g} + \frac{v_0^2}{g} + h_0 \\
0 = - \frac{1}{2}g\frac{x_f^2}{v_0^2}-\frac{v_0^2}{2g} + \frac{v_0^2}{g} + h_0 \\
0 = - \frac{1}{2}g\frac{x_f^2}{v_0^2}-\frac{v_0^2}{2g} + \frac{v_0^2}{g} + h_0 \\
\end{align*}



\begin{align*}
v_0 = \sqrt{2g(H-h_0)} \\
v_0^2 = 2g(H-h_0) \\
0 = - \frac{1}{2}g\frac{x_f^2}{v_0^2}-\frac{v_0^2}{2g} + \frac{v_0^2}{g} + h_0 \\
\end{align*}


\begin{align*}
0 = \frac{-x_f^2}{4(H-h_0)}-(H-h_0) + 2(H-h_0) + h_0 \\
0 = \frac{-x_f^2}{4(H-h_0)}+(H-h_0) + h_0 \\
0 = \frac{-x_f^2}{4(H-h_0)}+H \\
-H = \frac{-x_f^2}{4(H-h_0)} \\
\frac{-H}{4(H-h_0)} = -x_f^2 \\
x_f^2 = \frac{H}{4(H-h_0)} \\
x_f = \sqrt{\frac{H}{4(H-h_0)}} \\

\end{align*}

# We can now apply the quadratic equation $\frac{-b \pm \sqrt{b^2 - 4ac}}{2a}$

# $x_0 = \frac{- \frac{\sin \theta}{\cos \theta} + \sqrt{ \frac{\sin^2 \theta}{\cos^2 \theta}  + 2gh_0\frac{1}{v_0^2\cos^2\theta}}}{-g\frac{1}{v_0^2\cos^2\theta}}$
