#+TITLE: Translational & Rotational KE
#+SUBTITLE: Advanced Mechanics
#+AUTHOR: David Freifeld

* Problem 1
#+BEGIN_LATEX
\thispagestyle{empty}
#+END_LATEX

\begin{align*}
\text{KE}_\text{total} = \sum_{i=1}^N \frac{1}{2} m_i (v_i \cdot v_i) \\
\text{KE}_\text{total} =  \sum_{i=1}^N \frac{1}{2} m_i (\vec{V}_\text{CM} + \vec{v}_i^{\text{ }\prime})^2 \\
\text{KE}_\text{total} =  \sum_{i=1}^N \frac{1}{2} m_i (\vec{V}_\text{CM}^2 + 2\vec{V}_\text{CM}{v}_i^{\text{ }\prime} + (\vec{v}_i^{\text{ }\prime})^2) \\
\text{KE}_\text{total} =  \sum_{i=1}^N \left( \frac{1}{2} m_i \vec{V}_\text{CM}^2 + m_i \vec{V}_\text{CM}\vec{v}_i^{\text{ }\prime} + \frac{1}{2} m_i (\vec{v}_i^{\text{ }\prime})^2 \right) \\
\text{KE}_\text{total} =  \sum_{i=1}^N \frac{1}{2} m_i \vec{V}_\text{CM}^2 +  \sum_{i=1}^N  m_i \vec{V}_\text{CM}\vec{v}_i^{\text{ }\prime} + \sum_{i=1}^N \frac{1}{2} m_i  (\vec{v}_i^{\text{ }\prime})^2 \\
\text{KE}_\text{total} =  \frac{1}{2} \vec{V}_\text{CM}^2 \sum_{i=1}^N m_i  + \vec{V}_{\text{CM}} \sum_{i=1}^N  m_i \vec{v}_i^{\text{ }\prime}  + \sum_{i=1}^N \frac{1}{2} m_i  (\vec{v}_i^{\text{ }\prime})^2 \\
\text{Define $M = \sum_{i=1}^N  m_i$.} \\
\vec{r}_\text{CM}^{\text{ }\prime} = \frac{1}{M} \sum_i m_i \vec{r}_i \\
\text{$\vec{r}_\text{CM}^{\text{ }\prime} = 0$ by definition (it is relative to itself).} \\
0 = \frac{1}{M} \sum_i m_i \vec{r}_i \\
\text{Differentiate with respect to time.} \\
0 = \frac{1}{M} \sum_i m_i \vec{v}_i \\
0 = \sum_i m_i \vec{v}_i \\
\text{Eliminate the middle term $ \vec{V}_{\text{CM}} \sum_{i=1}^N  m_i \vec{v}_i^{\text{ }\prime}$ as it is equal to 0.} \\
\text{KE}_\text{total} =  \frac{1}{2} \vec{V}_\text{CM}^2 \sum_{i=1}^N m_i  + \sum_{i=1}^N \frac{1}{2} m_i  (\vec{v}_i^{\text{ }\prime})^2 \\
\boxed{\text{KE}_\text{total} =  \frac{1}{2} M \vec{V}_\text{CM}^2  + \sum_{i=1}^N \frac{1}{2} m_i  (\vec{v}_i^{\text{ }\prime})^2} \\
\end{align*} 


