#+TITLE: Ball Launcher
#+AUTHOR: Houjun Liu

#+DOWNLOADED: screenshot @ 2021-09-19 17:29:09
#+ATTR_ORG: :width 400
[[file:2021-09-19_17-29-09_screenshot.png]]

* Setup
The ball launcher problem involves an energetic optimization to figure, given the situation as shown in the above image, the parameters $h_0$ and $\theta_0$ that would best create a maximum launch distance $x_f$.

In this problem, we will define the axis such that the "lower-left" corner of the wood block (corner sharing $x$ value of the starting position of the marble, but on the "ground") as $(-w,0)$, where $w$ is the width of the wooden block. Therefore, we derive the x-value of the location of the launch of the projectile as $x=0$. We define the direction towards with the marble is launching as positive-x, so as the marble rolls, its position's $x$ value increases. We will define the location of the marble before starting as positive $y$, and as the marble decreases in height, its position's $y$ value decreases.

We define the start of the experiment as time $t_0$, the moment the marble leaves the track and travels as a projectile as $t_1$, and the end --- in the moment when the marble hits the ground --- as $t_f$. We will call the marble $m_0$.

* Figuring the Velocity at $t_1$
In order to expedite the process of derivation, we will leverage an energetic argument instead of that of kinematics for figuring the velocity at launch. The change-in-height that $m_0$ experiences before $t_1$ is $\Delta h = H-h_0$. Therefore, the potential energy expenditure is $\Delta PE_{grav} = mg\Delta h = m_0 g (H - h_0)$. Assuming that the marble starts out with 0 kinetic energy, we deduct that, at the moment of it finishing its descent, it will possess kinetic energy $KE = 0+m_0 g (H - h_0) = m_0 g (H - h_0)$.

For this derivation, for now, we ignore $KE_{rotational}$, hence, we could roughly deduct the statement that $KE_{translational} \approx m_0 g (H - h_0)$.

Creating this statement, we could deduct a statement that we could leverage to solve for the velocity at $t_1$ named $\vec{v_0}$.

\begin{align}
    m_0g(H-h_0) =& \frac{1}{2}m_0\vec{v_0}^2 \\
    g(H-h_0) =& \frac{1}{2}\vec{v_0}^2 \\
    2g(H-h_0) =& \vec{v_0}^2 \\
    \vec{v_0} =& \sqrt{2g(H-h_0)}
\end{align}

This velocity vector could be easily split into its two constituent parts. Namely:

\begin{equation}
    \begin{cases}
        \vec{v_0_x} = \sqrt{2g(H-h_0)}cos(\theta_0)\\
        \vec{v_0_y} = \sqrt{2g(H-h_0)}sin(\theta_0)\\
    \end{cases}
\end{equation}

* Figuring the Maximum Possible Travel Distance
Here, we devise an function for $x_f$ w.r.t. $\vec{v_0_y}$, $\vec{v_0_x}$, $h_0$, $m_0$.

** Setup for Kinematics
We first will leverage the parametric equations for position in kinematics in order to ultimately result in a function for $x_f$.

\begin{equation}
    \begin{cases}
        x(t) = \frac{1}{2}a_0_xt^2 + v_0_xt + x_0 \\
        y(t) = \frac{1}{2}a_0_yt^2 + v_0_yt + y_0 \\
    \end{cases}
\end{equation}

Given the situation of our problem, we could modify the pair as follows:

\begin{equation}
    \begin{cases}
        x(t) = v_0_xt \\
        y(t) = \frac{1}{2}gt^2 + v_0_yt + h_0 \\
    \end{cases}
\end{equation}

as...

- there are no acceleration in the x-direction at the point of launch
- the only acceleration in the y-direction is that due to gravity
- the start x-position of the marble at launch is, as defined above, $x=0$
- the start y-position of the marble at launch is, as defined above, $y=h_0$

** Solving for $x_f$
The position equations above could be leveraged to figure a value for $x_f$. We first create a set of equations modeling the location of the marble at $t_f$.

\begin{equation}
    \begin{cases}
        x(t_f) = x_f = v_0_xt_f = t_f\sqrt{2g(H-h_0)}cos(\theta_0)\\
        y(t_f) = 0 = \frac{1}{2}g{t_f}^2 + v_0_y t_f + h_0 = \frac{1}{2}g{t_f}^2 +  t_f\sqrt{2g(H-h_0)}sin(\theta_0) + h_0
    \end{cases}
\end{equation}


To simplify calculations initially, we set $\sqrt{2g(H-h_0})$  back as $v

# To combine the two expressions, we perform variable substitution upon $\sqrt{2g(H-h_0)}$.

# We first prepare the first expression to achieve this:

# \begin{align}
#     x_f =& t_f \sqrt{2g(H-h_0)}cos(\theta_0) \\
# \Rightarrow x_f =& t_f \sqrt{2g(H-h_0)}cos(\theta_0) \\
# \Rightarrow \sqrt{2g(H-h_0)} =& \frac{x_f}{t_f cos(\theta_0)} \\
# \end{align}
# With this statement, we perform the actual substitution.

# \begin{align}
#     0 =& \frac{1}{2}g{t_f}^2 + t_f\sqrt{2g(H-h_0)}sin(\theta_0) + h_0 \\
# \Rightarrow 0 =& \frac{1}{2}g{t_f}^2 + t_f\sqrt{2g(H-h_0)}sin(\theta_0) + h_0 \\
# \Rightarrow 0 =& \frac{1}{2}g{t_f}^2 + t_f\frac{x_f}{t_f cos(\theta_0)} sin(\theta_0) + h_0 \\
# \Rightarrow 0 =& \frac{1}{2}g{t_f}^2 + x_ftan(\theta_0) + h_0 \\
# \end{align}

# And finally, we solve for $x_f$ within this expression.

# \begin{align}
#     0 =& \frac{1}{2}g{t_f}^2 + x_ftan(\theta_0) + h_0 \\
#     \Rightarrow -\frac{1}{2}g{t_f}^2 - h_0 =& x_ftan(\theta_0) \\
#     \Rightarrow x_f =& \frac{-(\frac{1}{2}g{t_f}^2 + h_0)}{tan(\theta_0)} 
# \end{align}

# We then proceed to isolate $t_f$ from the first expression and performing substitution again.

# \begin{align}
#     x_f = t_f\sqrt{2g(H-h_0)}cos(\theta_0)\\
#     t_f = \frac{x_f}{\sqrt{2g(H-h_0)}cos(\theta_0)}\\
# \end{align}
# We then perform the final substitution

# \begin{align}
#     x_f =& \frac{-(\frac{1}{2}g{\frac{x_f}{\sqrt{2g(H-h_0)}cos(\theta_0)}}^2 + h_0)}{tan(\theta_0)} \\
#     =& \frac{-(\frac{1}{2}g{\frac{{x_f}^2}{2g(H-h_0)cos^2(\theta_0)}} + h_0)}{tan(\theta_0)} \\
#     =& \frac{-({\frac{{x_f}^2}{4(H-h_0)cos^2(\theta_0)}} + h_0)}{tan(\theta_0)} \\
#     =& \frac{{\frac{{x_f}^2}{4(H-h_0)cos^2(\theta_0)}} - h_0}{tan(\theta_0)} \\
#     x_f tan(\theta_0) =& \frac{{x_f}^2}{4(H-h_0)cos^2(\theta_0)} - h_0 \\
# \end{align}





