:PROPERTIES:
:ID:       4BBC4863-78B9-484F-B8B9-33A1B2ACFA74
:END:
#+title: Newton's Laws Pulleys
#+author: Houjun Liu

* Pulley Problem

** Number 1
Three tie points, tied onto one point.

\begin{align}
&3T_1 = T\\
\Rightarrow &T_1 = \frac{1}{3}T
\end{align}

#+DOWNLOADED: screenshot @ 2022-02-03 10:01:45
[[file:2022-02-03_10-01-45_screenshot.png]]


** Number 2
Three tie points, tied onto one point. The extra additional pull, given its not tied, simply transfers tension.

\begin{align}
&3T_1 = T\\
\Rightarrow &T_1 = \frac{1}{3}T
\end{align}


#+DOWNLOADED: screenshot @ 2022-02-03 10:01:52
[[file:2022-02-03_10-01-52_screenshot.png]]


** Number 3
Five points, tied onto one point. 

\begin{align}
&5T_1 = T\\
\Rightarrow &T_1 = \frac{1}{5}T
\end{align}


#+DOWNLOADED: screenshot @ 2022-02-03 10:02:01
[[file:2022-02-03_10-02-01_screenshot.png]]


** Number 4
Two tie points on one, which is added to another set of tie points. The higher (smaller) set has a total tension of $3T_1$, which is tied again onto the bottom tie point.

\begin{align}
&9T_1 = T\\
\Rightarrow &T_1 = \frac{1}{9}T
\end{align}


#+DOWNLOADED: screenshot @ 2022-02-03 10:02:44
[[file:2022-02-03_10-02-44_screenshot.png]]


** Number 5
The top tie point has $3T_1$ of tension. The bottom has $2T_1$, and they are finally all added together.

\begin{align}
&3T_1 + 2T_1 = T\\
\Rightarrow &T_1 = \frac{1}{5}T
\end{align}


#+DOWNLOADED: screenshot @ 2022-02-03 10:02:51
[[file:2022-02-03_10-02-51_screenshot.png]]


** Number 6
The top tie point has $3T_1$ of tensions, and the bottom has four tie points and tied together towards the bottom. 

\begin{align}
&3T_1 + 4T_1 = T\\
\Rightarrow &T_1 = \frac{1}{7}T
\end{align}


#+DOWNLOADED: screenshot @ 2022-02-03 10:03:00
[[file:2022-02-03_10-03-00_screenshot.png]]


** Number 7
The top tie point has $2T_1$ of ties, the bottom has $3T_1$, which is finally tied to another propagated to another $6T_1$ tie point. In total, therefore:

\begin{align}
&2T_1 + 3T_1 + 6T_1 = T\\
\Rightarrow &T_1 = \frac{1}{11}T
\end{align}


#+DOWNLOADED: screenshot @ 2022-02-03 10:03:05
[[file:2022-02-03_10-03-05_screenshot.png]]

* Sliding Blocks

#+DOWNLOADED: screenshot @ 2022-02-03 11:40:21
[[file:2022-02-03_11-40-21_screenshot.png]]

Given the masses $M_a$, $M_b$, $F_f$ between them, and $A$ the acceleration of the pully pulling them, we are to figure the tension $T$ on the rope.

We will first draw free-body diagrams of each of the objects, like so:


#+DOWNLOADED: screenshot @ 2022-02-03 11:41:33
[[file:2022-02-03_11-41-33_screenshot.png]]


#+DOWNLOADED: screenshot @ 2022-02-03 11:41:36
[[file:2022-02-03_11-41-36_screenshot.png]]

We will note that, given $M_b > M_a$, $M_a$ will slide to the "right" (+x) direction. As such, in the reference frame of $M_a$, the force of friction is in the opposite direction as $T$, whereas this is the opposite case for $M_b$.

According to these free-body diagrams, then, we can conclude that:

\begin{equation}
    \begin{cases}
    M_a a_a = T- F_f \\
M_b a_b = T+ F_f
\end{cases}
\end{equation}

As we have three unknowns and two expressions, we have one remaining degree of freedom to address. This can be analysed by looking at the rope connecting $M_a$ and $M_b$.

We will define the position of $M_a$ as $x_a$, $M_b$ as $x_b$, and finally the position of the pulley as $x_p$. We will further introduce a temporary constant value $L$ representing the length of the perfect rope connecting the two blocks.

We can, therefore, claim that:

\begin{equation}
   (x_p - x_a) + (x_p-x_b) = L
\end{equation}

That the two distances from block to pulley added up is the length of the rope.

Performing slight algebraic simplifications:

\begin{align}
&(x_p-x_a)+(x_p-x_b) = L \\
\Rightarrow & 2x_p-(x_a+x_b) = L \\
\Rightarrow & 2x_p = L +(x_a+x_b)\\
\Rightarrow & x_p = \frac{L +(x_a+x_b)}{2}
\end{align}

We can now take two derivatives w.r.t. time:

\begin{equation}
   \frac{d^2x_p }{d{t^2}} = \frac{\ddot{x_a}+\ddot{x_b}}{2}
\end{equation}

And, therefore:

\begin{equation}
    A = \frac{{a_a}+{a_b}}{2}
\end{equation}

We now have three unknowns and three equations, which therefore allows for solving:

\begin{equation}
    \begin{cases}
    M_a a_a = T- F_f \\
M_b a_b = T+ F_f\\
A = \frac{{a_a}+{a_b}}{2}
\end{cases}
\end{equation}

Solving for the equations above symbolically, we arrive at the following expressions:

\begin{equation}
\left[a_{a} = \frac{2 \, {\left(A M_{b} - F_{f}\right)}}{M_{a} + M_{b}}, a_{b} = \frac{2 \, {\left(A M_{a} + F_{f}\right)}}{M_{a} + M_{b}}, T = \frac{{\left(2 \, A M_{b} - F_{f}\right)} M_{a} + F_{f} M_{b}}{M_{a} + M_{b}}\right]
\end{equation}

The value for tension, therefore, is the last expression highlighted above.
