:PROPERTIES:
:ID:       C19AABA7-293A-4EEE-B089-442D55E1FB58
:END:
#+TITLE: Torque Number 3
#+AUTHOR: Houjun Liu

* External Torque

Proof:

\begin{equation}
\vec{\tau}_{total\ ext} = \frac{d \vec{L}_{system}}{dt}
\end{equation}

According to the work that is already done, we have that:

\begin{equation}
   \frac{d \vec{L}_{system}}{dt} = \vec{\tau}_{tot\ ext} + \sum_{1 \leq i < j \leq N} \left[ (\vec{r}_i \times \vec{F}_{j \to i}) + (\vec{r}_j \times \vec{F}_{i \to j}) \right]
\end{equation}

The left expression $\vec{\tau}_{tot\ ext}$ already achieves what we want in terms of the final expression, so the right expression must cancel to $0$. 

We first begin by recognizing, by Newton's Third Law, $\vec{F}_{i\to j} = -\vec{F}_{j\to i}$ as long as both objects are within the system. Therefore, we will first begin by making this substitution below:

\begin{align}
(\vec{r}_i \times \vec{F}_{j \to i}) + (\vec{r}_j \times \vec{F}_{i \to j}) =  (\vec{r}_j \times \vec{F}_{i \to j}) -(\vec{r}_i \times \vec{F}_{i \to j})
\end{align}

We further understand that the cross-product is distributive across addition; therefore:

\begin{align}
(\vec{r}_i \times \vec{F}_{j \to i}) + (\vec{r}_j \times \vec{F}_{i \to j}) &=  (\vec{r}_j \times \vec{F}_{i \to j}) -(\vec{r}_i \times \vec{F}_{i \to j})\\
&= (\vec{r}_j-\vec{r_i}) \times \vec{F}_{i \to j}
\end{align}

At this point, we realise that a vector $\vec{r_i}$ subtracted from $\vec{r_j}$ is a vector $i \to j$, which would be parallel to $\vec{F}_{i \to j}$. As such, their cross products would be zero.

Completing the proof, then:

\begin{align}
   \frac{d \vec{L}_{system}}{dt} &= \vec{\tau}_{tot\ ext} + \sum_{1 \leq i < j \leq N} \left[ (\vec{r}_i \times \vec{F}_{j \to i}) + (\vec{r}_j \times \vec{F}_{i \to j}) \right] \\
&= \vec{\tau}_{tot\ ext} + \sum_{1 \leq i < j \leq N} 0 \\
&= \vec{\tau}_{tot\ ext} + 0 \\
&= \vec{\tau}_{tot\ ext}\ \blacksquare
\end{align}

[[./2022-03-01_14-44-25_screenshot.png]]


* Two Rotating Point Masses
We do this problem by calculating the angular momentum of each of the $m_{\{1,2\}}$, and adding the angular accelerations together.

The system is given by this figure:

#+DOWNLOADED: screenshot @ 2022-03-03 22:44:48
[[file:2022-03-03_22-44-48_screenshot.png]]

We define a coordinate such that the "figure"'s left is the negative y direction, the "figure"'s right is the positive y direction. The side "outside" the page is the positive x direction, and the side "inside" the page is the negative x direction.

** Angular Momentum from $m_1$
We begin with the expression for tangential velocity, which is simply $R \omega$.

Therefore:

\begin{align}
   \vec{V} &= (R\hat{j})(\omega \hat{k}) \\
&=(R\omega) (\hat{j}\hat{k})\\
&=R\omega \hat{i}
\end{align}

We will supply this expression for that of the angular momentum: $\vec{R} \times m\vec{V}$:

\begin{align}
   \vec{L} &= \vec{r} \times m\vec{V} \\
&=(-R\hat{j} + h\hat{k}) \times m(R\omega \hat{i})\\
&=-R\hat{j}\times mR\omega \vec{i} + h\hat{k}\times mR\omega \vec{i} \\
&=-mR^2\omega (\hat{j}\times\hat{i}) + h mR\omega (\hat{k}\times\hat{i}) \\
&=mR^2\omega \hat{k} + h mR\omega \hat{j} 
\end{align}

** Angular Momentum from $m_2$
The calculations here is essentially almost the same. We just need to take a few sign changes as $R$ in $m_2$ is in the opposite direction as $R$ in $m_1$.

Therefore:

\begin{align}
   \vec{V} &= (-R\hat{j})(\omega \hat{k}) \\
&=(-R\omega) (\hat{j}\hat{k})\\
&=-R\omega \hat{i}
\end{align}

And, as with before, we supply it to the previous expression.

\begin{align}
   \vec{L} &= \vec{r} \times m\vec{V} \\
&=(R\hat{j} + h\hat{k}) \times m(-R\omega \hat{i})\\
&=R\hat{j}\times -mR\omega \vec{i} + h\hat{k}\times -mR\omega \vec{i} \\
&=-mR^2\omega (\hat{j}\times\vec{i}) - h mR\omega (\hat{k}\times\vec{i}) \\
&=mR^2\omega \hat{k} - h mR\omega \hat{j} 
\end{align}

** Summing the $\vec{L_i}$ s
We will now sub the two $\vec{L_i}$ s together:

\begin{align}
   \vec{L}_1 + \vec{L}_2 &= mR^2\omega \hat{k} + h mR\omega \hat{j} +mR^2\omega \hat{k} - h mR\omega \hat{j} \\
&= mR^2\omega \hat{k} +mR^2\omega \hat{k} + h mR\omega \hat{j}  - h mR\omega \hat{j}\\
&= 2mR^2\omega \hat{k} + 0\\
&= 2mR^2\omega \hat{k}\ \blacksquare
\end{align}

* Rigid Body Generalization 

** N-Mass Formula
We will think about a single mass $m_i$ in isolation. We will use $\ell_i$ to represent the perpendicular distance from $m_i$ to $\hat{k}$. 

We begin by analyzing some $m_i$, and add all $m_i$ together.

** The angular momentum of $m_i$
For every object $m_i$, we take it being arranged at some $\theta$ between $\hat{i}$ and $\hat{j}$. We will perform the same procedures as with above to calculate angular momentum.

$\ell_i$ is angled between $\hat{i}$ and $\hat{j}$. Specifically, it is located at:

\begin{equation}
   \ell_i = cos(\theta) \ell_i\hat{i} + sin(\theta) \ell_i\hat {j} 
\end{equation}

We will calculate the tangential velocity, as usual:

\begin{align}
   \vec{V} &= (cos(\theta) \ell_i\hat{i} + sin(\theta) \ell_i\hat {j})(\omega \hat{k}) \\
&= cos(\theta)\ell_i(\omega \hat{k}) \hat{i} + sin(\theta)\ell_i(\omega \hat{k}) \hat {j}\\
&= cos(\theta)\ell_i\omega (\hat{k} \hat{i}) + sin(\theta)\ell_i\omega (\hat{k} \hat {j})\\
&= cos(\theta)\ell_i\omega \hat{j} - sin(\theta)\ell_i\omega \hat{i}
\end{align}

And, as with before, we will supply it to the expression for angular momentum. 

\begin{align}
   \vec{L} &= \vec{r} \times m\vec{V} \\
&=(cos(\theta)\ell_i \hat{i} + sin(\theta)\ell_i \hat {j} + h\hat{k}) \times m(cos(\theta)\ell_i\omega \hat{j} - sin(\theta)\ell_i\omega \hat{i})\\
&=(cos(\theta)\ell_i \hat{i} + sin(\theta)\ell_i \hat {j} + h\hat{k}) \times (mcos(\theta)\ell_i\omega \hat{j} - msin(\theta)\ell_i\omega \hat{i})
\end{align}

We will now compute the actual cross product:

\begin{align}
   \vec{L} = &(hmcos\theta \ell_i \omega) \hat{i}  +\\
&(hmsin\theta\ell_i \omega)\hat{j} +\\
&(m\omega(cos\theta \ell_i)^2 + m\omega(sin\theta \ell_i)^2)\hat{k}
\end{align}

Let's expand the last term slightly:

\begin{align}
  &m\omega(cos\theta \ell_i)^2 + m\omega(sin\theta \ell_i)^2\\
=&m\omega(cos\theta \ell_i)^2 + m\omega(sin\theta \ell_i)^2\\
=&m\omega\ cos^2\theta {\ell_i}^2 + m\omega\ sin^2 \theta {\ell_i}^2\\
=&m\omega(1-sin^2\theta) {\ell_i}^2 + m\omega\ sin^2 \theta {\ell_i}^2 \\
=&m\omega{\ell_i}^2- m\omega{\ell_i}^2sin^2\theta + m\omega\ sin^2 \theta {\ell_i}^2 \\
=&m\omega{\ell_i}^2
\end{align}

And therefore, we can re-write the following expression for $\vec{L}$:

\begin{align}
   \vec{L} = &(hmcos\theta \ell_i \omega) \hat{i}  +\\
&(hmsin\theta\ell_i \omega)\hat{j} +\\
&m\omega{\ell_i}^2\hat{k}
\end{align}

** Angular momentum of the system

Therefore, the total momentum of the system would be:

\begin{align}
       \vec{L} = \sum^N_{i=1} \left(hm\ cos\left(\frac{2\pi i}{N}\right) \ell_i \omega\right) \hat{i}  +\left(hm\ sin\left(\frac{2\pi i}{N}\right)\ell_i \omega\right)\hat{j} +m\omega{\ell_i}^2\hat{k}
\end{align}

At this point, we need to remember the fact that the points in the generalized formula we are to derive are axially symmetric. This means that the components $cos{\theta} \hat{i}$ and $sin(\theta)\hat{j}$ will, pairwise, cancel each other out.

\begin{align}
       \vec{L} &= \sum^N_{i=1} \left(hm\ cos\left(\frac{2\pi i}{N}\right) \ell_i \omega\right) \hat{i}  +\left(hm\ sin\left(\frac{2\pi i}{N}\right)\ell_i \omega\right)\hat{j} +m\omega{\ell_i}^2\hat{k}\\
&=\sum^N_{i=1} 0 +m\omega{\ell_i}^2\hat{k}\\
&=\sum^N_{i=1} m\omega{\ell_i}^2\hat{k}\\
&=\hat{k}\omega\sum^N_{i=1} m{\ell_i}^2
\end{align}

** Actual Integral Expression
Our object has total mass $M$ and volume $V_0$. We will now determine an integral expression for its angular momentum.

So far, we have that:

\begin{equation}
 \vec{L}=\hat{k}\omega\sum^N_{i=1} m{\ell_i}^2
\end{equation}

We will convert $\ell_i = \ell(m)$, a function in terms of differential mass $m$ that maps mass to the distance from $z$ axis $\ell$.

Hence:

\begin{align}
 \vec{L}&=\hat{k}\omega\sum^N_{i=1} m{\ell_i}^2\\
&=\hat{k}\omega\int_V {\ell}^2dm\\
&=\hat{k}\omega\int_V {\ell}^2\frac{dm}{dv} dV\\
&=\hat{k}\omega\int_V {\ell}^2\frac{M}{V_0} dV
\end{align}

In our last step, we can see that the ratio between differential $\frac{dm}{dv}$ can be equivalent---as all components of this system are point masses---to the overall $\frac{M}{V_0}$.

* The Rod
In this problem, we essentially have a line of aligned infinitesimal point masses around the -center.

For every point $i$, we understand that its tangential velocity can be modeled by:

\begin{align}
   \vec{V} &= (\ell_i\hat{j})(\omega \hat{k}) \\
&=(\ell_i\omega) (\hat{j}\hat{k})\\
&=\ell_i\omega \hat{i}
\end{align}

We again supply this expression into that for $\vec{L}$:

\begin{align}
   \vec{L_i} &= \vec{r} \times m_i\vec{V} \\
&=(\ell_i \hat{j} + h\hat{k}) \times m_i \ell_i \omega \hat{i}\\
&=\ell_i  m_i \ell_i \omega (\hat{j}\times \hat{i}) + h m_i \ell_i \omega (\hat{k}\times\hat{i})\\
&= -h m_i \ell_i \omega \hat{j}+{\ell_i}^2 m_i \omega \hat{k}
\end{align}

To figure the actual momentum, we will have to sum the momentums for all $i$:

\begin{equation}
   \vec{L} = \sum_i \vec{L_i} = \sum_i \left(-h m_i \ell_i \omega \hat{j}+{\ell_i}^2 m_i \omega \hat{k}\right)
\end{equation}

Of course, to actually perform the summation, we integrate over each differential mass:

\begin{align}
    &\int_L \left(-h \ell \omega \hat{j}+\ell^2 \omega \hat{k}\right) dm\\
=&\omega \int_L \left(-h\ell \hat{j}+\ell^2 \hat{k}\right) dm\\
=&\omega \int_L \left(-h\ell \hat{j}+\ell^2 \hat{k}\right) \frac{dm}{dl} dl\\
=&\omega \int_L \left(-h\ell \hat{j}+\ell^2 \hat{k}\right) \lambda dl\\
=&\omega \lambda \int_L \left(- h\ell \hat{j}+\ell^2 \hat{k}\right) dl
\end{align}

We now supply the integral with actual bounds: $[-\frac{L}{2}, \frac{L}{2}]$.

\begin{align}
&\omega  \lambda\int_L \left(- h\ell \hat{j}+\ell^2 \hat{k}\right) dl \\
=&\omega  \lambda\int_{-\frac{L}{2}}^{\frac{L}{2}} \left( -h\ell \hat{j}+\ell^2 \hat{k}\right) dl \\
=&\omega  \lambda  \left(\int_{-\frac{L}{2}}^{\frac{L}{2}}-h\ell \hat{j}dl+\int_{-\frac{L}{2}}^{\frac{L}{2}}\ell^2 \hat{k} dl \right)\\
=&\omega  \lambda  \left(h\hat{j}\int_{-\frac{L}{2}}^{\frac{L}{2}}\ell dl-\hat{k}\int_{-\frac{L}{2}}^{\frac{L}{2}}\ell^2  dl \right)\\
=&\omega  \lambda  \left\left(-h\hat{j}\frac{\ell^2}{2} +\hat{k}\frac{\ell^3}{3}  \right)\right|_{-\frac{L}{2}}^{\frac{L}{2}}\\
=&\omega  \lambda  \left(-h\hat{j}\frac{\frac{L}{2}^2}{2} +\hat{k}\frac{\frac{L}{2}^3}{3}  \right)-\left(-h\hat{j}\frac{\frac{-L}{2}^2}{2} +\hat{k}\frac{\frac{-L}{2}^3}{3}  \right)\\
=& 2\frac{L^3}{24} \omega  \lambda   \hat{k}\\
=& \frac{L^3}{12} \omega  \lambda   \hat{k}
\end{align}

We continue be realizing that $\lambda = \frac{M}{L}$. Supplying that to the equation:

\begin{align}
& \frac{L^3}{12} \omega  \lambda   \hat{k} \\
=& \frac{L^3}{12} \omega  \frac{M}{L} \hat{k} \\
=& \frac{L^2}{12} M \omega  \hat{k} \\
=& \frac{1}{12}L^2M \omega  \hat{k} 
\end{align}

* The Disk
Our original expression for the momentum in the system is the same. 

\begin{align}
   \vec{L_i} &= \vec{r} \times m_i\vec{V} \\
&=m\omega{\ell_i}^2\hat{k}
\end{align}

We will have to add the angular momentum in two directions to get that of a disk:

\begin{equation}
   \vec{L} = \sum_i \vec{L_i} = \sum_A \vec{L_i}
\end{equation}

where, $A$ is the area of the surface.

To begin doing this, we will construct the differential operator for a disk. We understand the circumference of the circle is $2 \pi r$ for some radius r. Furthermore, for a small ring with infinitesimal thickness $dr$, it has an area of $2\pi r dr$.

Therefore:

\begin{equation}
    da = 2\pi r dr
\end{equation}

We finally want to find the expression for differential mass. Of course, it is simply the mass density $\frac{dm}{da}$ multiplied by the value of $da$.

\begin{align}
   dm &= \frac{dm}{da}\ da\\
&= \sigma\ da \\
&= \frac{M}{\pi R^2} da\\
&= \frac{M}{\pi R^2} 2\pi r dr\\
&= \frac{2 rM}{R^2} dr
\end{align}

We can now finally take the integral:

\begin{align}
   &\int_{0}^{R} \vec{L}_i  \\
\Rightarrow &\int_{0}^{R} \omega r^2\hat{k}\ dm\\
\Rightarrow &\int_{0}^{R} \omega r^2\hat{k} \frac{2 rM}{R^2} dr\\
\Rightarrow &\int_{0}^{R} \omega \hat{k} \frac{2 r^3M}{R^2} dr\\
\Rightarrow &\frac{2 M \omega }{R^2} \hat{k}\int_{0}^{R}  r^3 dr\\
\Rightarrow &\frac{2 M \omega }{R^2} \hat{k} \left(\left\frac{r^4}{4}\right|_0^R\right)\\
\Rightarrow &\frac{2 M \omega }{R^2} \hat{k} \frac{R^4}{4}\\
\Rightarrow &\frac{1}{2}MR^2 \omega \hat{k}\ \blacksquare
\end{align}

